added limited export

lib/DataStructures/MutableBtree.i.dfy
@@ -4,18 +4,22 @@ include "../Base/total_order.i.dfy"
 include "../Base/sequences.i.dfy"
 include "../Base/Arrays.i.dfy"
 include "../Base/Maps.s.dfy"
+include "../Base/Option.s.dfy"
 include "BtreeSpec.i.dfy"
 
 abstract module MutableBtree {
   import opened NativeTypes
   import opened NativeArrays
   import opened Seq = Sequences
+  import opened Options
   import opened Maps
   import Arrays
-  import BS : BtreeSpec
+  import Spec : BtreeSpec
+
+  export API provides WF, Interpretation, EmptyTree, Insert, Query, NativeTypes, Spec, Options reveals Node, NodeContents, Key, Value
   
-  type Key = BS.Keys.Element
-  type Value = BS.Value
+  type Key = Spec.Keys.Element
+  type Value = Spec.Value
 
   function method MaxKeysPerLeaf() : uint64
     ensures 1 < MaxKeysPerLeaf() as int < Uint64UpperBound() / 2
@@ -31,10 +35,11 @@ abstract module MutableBtree {
     ghost var repr: set<object>
     ghost var height: nat
   }
-    
+  
   datatype NodeContents =
     | Leaf(nkeys: uint64, keys: array<Key>, values: array<Value>)
     | Index(nchildren: uint64, pivots: array<Key>, children: array<Node?>)
+
 
   predicate DisjointSubtrees(node: NodeContents, i: int, j: int)
     requires node.Index?
@@ -74,7 +79,7 @@ abstract module MutableBtree {
       && (forall i :: 0 <= i < node.contents.nchildren ==> WFShape(node.contents.children[i]))
   }
 
-  function Ichildren(nodes: seq<Node>, parentheight: int) : (result: seq<BS.Node>)
+  function Ichildren(nodes: seq<Node>, parentheight: int) : (result: seq<Spec.Node>)
     requires forall i :: 0 <= i < |nodes| ==> WFShape(nodes[i])
     requires forall i :: 0 <= i < |nodes| ==> nodes[i].height < parentheight
     ensures |result| == |nodes|
@@ -87,16 +92,16 @@ abstract module MutableBtree {
     else Ichildren(DropLast(nodes), parentheight) + [I(Last(nodes))]
   }
   
-  function I(node: Node) : (result: BS.Node)
+  function I(node: Node) : (result: Spec.Node)
     requires WFShape(node)
     reads node, node.repr
     decreases node.height
   {
     match node.contents {
-      case Leaf(nkeys, keys, values) => BS.Leaf(keys[..nkeys], values[..nkeys])
+      case Leaf(nkeys, keys, values) => Spec.Leaf(keys[..nkeys], values[..nkeys])
       case Index(nchildren, pivots, children) =>
         var bschildren := Ichildren(children[..nchildren], node.height);
-        BS.Index(pivots[..nchildren-1], bschildren)
+        Spec.Index(pivots[..nchildren-1], bschildren)
     }
   }
 
@@ -109,50 +114,52 @@ abstract module MutableBtree {
   }
 
   predicate WF(node: Node)
+    ensures WF(node) ==> node in node.repr
     reads node, node.repr
   {
     && WFShape(node)
-    && BS.WF(I(node))
+    && Spec.WF(I(node))
   }
 
   function Interpretation(node: Node) : map<Key, Value>
     requires WF(node)
-    reads node, node.repr
+    reads node.repr
   {
-    BS.Interpretation(I(node))
-  }  
-  
-  method QueryLeaf(node: Node, needle: Key) returns (result: BS.QueryResult)
+    Spec.Interpretation(I(node))
+  }
+    
+
+  method QueryLeaf(node: Node, needle: Key) returns (result: Option<Value>)
     requires WF(node)
     requires node.contents.Leaf?
-    ensures needle in BS.Interpretation(I(node)) ==> result == BS.Found(BS.Interpretation(I(node))[needle])
-    ensures needle !in BS.Interpretation(I(node)) ==> result == BS.NotFound
-    decreases node.height, 0
+    ensures needle in Interpretation(node) ==> result == Some(Interpretation(node)[needle])
+    ensures needle !in Interpretation(node) ==> result == None
+    decreases node.repr, 0
   {
-    var posplus1: uint64 := BS.Keys.ArrayLargestLtePlus1(node.contents.keys, 0, node.contents.nkeys, needle);
+    var posplus1: uint64 := Spec.Keys.ArrayLargestLtePlus1(node.contents.keys, 0, node.contents.nkeys, needle);
     if 1 <= posplus1 && node.contents.keys[posplus1-1] == needle {
-      result := BS.Found(node.contents.values[posplus1-1]);
+      result := Some(node.contents.values[posplus1-1]);
     } else {
-      result := BS.NotFound;
+      result := None;
     }
   }
 
-  method QueryIndex(node: Node, needle: Key) returns (result: BS.QueryResult)
+  method QueryIndex(node: Node, needle: Key) returns (result: Option<Value>)
     requires WF(node)
     requires node.contents.Index?
-    ensures needle in BS.Interpretation(I(node)) ==> result == BS.Found(BS.Interpretation(I(node))[needle])
-    ensures needle !in BS.Interpretation(I(node)) ==> result == BS.NotFound
-    decreases node.height, 0
+    ensures needle in Spec.Interpretation(I(node)) ==> result == Some(Spec.Interpretation(I(node))[needle])
+    ensures needle !in Spec.Interpretation(I(node)) ==> result == None
+    decreases node.repr, 0
   {
-    var posplus1: uint64 := BS.Keys.ArrayLargestLtePlus1(node.contents.pivots, 0, node.contents.nchildren-1, needle);
+    var posplus1: uint64 := Spec.Keys.ArrayLargestLtePlus1(node.contents.pivots, 0, node.contents.nchildren-1, needle);
     result := Query(node.contents.children[posplus1], needle);
   }
 
-  method Query(node: Node, needle: Key) returns (result: BS.QueryResult)
+  method Query(node: Node, needle: Key) returns (result: Option<Value>)
     requires WF(node)
-    ensures needle in BS.Interpretation(I(node)) ==> result == BS.Found(BS.Interpretation(I(node))[needle])
-    ensures needle !in BS.Interpretation(I(node)) ==> result == BS.NotFound
-    decreases node.height, 1
+    ensures needle in Interpretation(node) ==> result == Some(Interpretation(node)[needle])
+    ensures needle !in Interpretation(node) ==> result == None
+    decreases node.repr, 1
   {
     match node.contents {
       case Leaf(_, _, _) => result := QueryLeaf(node, needle);
@@ -173,13 +180,13 @@ abstract module MutableBtree {
     requires WF(node)
     requires node.contents.Leaf?
     requires 0 < nleft < node.contents.nkeys
-    requires BS.Keys.lt(node.contents.keys[nleft-1], pivot)
-    requires BS.Keys.lte(pivot, node.contents.keys[nleft])
+    requires Spec.Keys.lt(node.contents.keys[nleft-1], pivot)
+    requires Spec.Keys.lte(pivot, node.contents.keys[nleft])
     ensures WFShape(node)
     ensures WFShape(right)
     ensures node.repr == old(node.repr)
     ensures fresh(right.repr)
-    ensures BS.SplitLeaf(old(I(node)), I(node), I(right), wit, pivot)
+    ensures Spec.SplitLeaf(old(I(node)), I(node), I(right), wit, pivot)
     ensures node.contents.nkeys == nleft
     modifies node
   {
@@ -195,7 +202,7 @@ abstract module MutableBtree {
 
     node.contents := Leaf(nleft, node.contents.keys, node.contents.values);
     wit := node.contents.keys[0];
-    BS.Keys.IsStrictlySortedImpliesLt(old(node.contents.keys[..node.contents.nkeys]), nleft as int - 1, nleft as int);
+    Spec.Keys.IsStrictlySortedImpliesLt(old(node.contents.keys[..node.contents.nkeys]), nleft as int - 1, nleft as int);
   }
 
   predicate ObjectIsInSubtree(node: Node, o: object, i: int)
@@ -307,7 +314,7 @@ abstract module MutableBtree {
     ensures WFShape(node)
     ensures node.repr == old({node, node.contents.pivots, node.contents.children} + SubRepr(node, 0, newnchildren as int))
     ensures node.height == old(node.height)
-    ensures I(node) == BS.SubIndex(old(I(node)), 0, newnchildren as int)
+    ensures I(node) == Spec.SubIndex(old(I(node)), 0, newnchildren as int)
     modifies node
   {
     ghost var oldinode := I(node);
@@ -320,7 +327,7 @@ abstract module MutableBtree {
       assert old(DisjointSubtrees(node.contents, i, j));
     }
     ghost var newinode := I(node);
-    assert newinode == BS.SubIndex(oldinode, 0, newnchildren as int);
+    assert newinode == Spec.SubIndex(oldinode, 0, newnchildren as int);
   }
 
   method SubIndex(node: Node, from: uint64, to: uint64) returns (subnode: Node)
@@ -332,7 +339,7 @@ abstract module MutableBtree {
     ensures subnode.contents.Index?
     ensures subnode.repr == SubRepr(node, from as int, to as int) + {subnode, subnode.contents.pivots, subnode.contents.children}
     ensures subnode.height == node.height
-    ensures I(subnode) == BS.SubIndex(I(node), from as int, to as int)
+    ensures I(subnode) == Spec.SubIndex(I(node), from as int, to as int)
     ensures fresh(subnode)
     ensures fresh(subnode.contents.pivots)
     ensures fresh(subnode.contents.children)
@@ -400,7 +407,7 @@ abstract module MutableBtree {
     ensures node.repr !! right.repr
     ensures fresh(right.repr - old(node.repr))
     ensures node.height == old(node.height) == right.height
-    ensures BS.SplitIndex(old(I(node)), I(node), I(right), wit, pivot)
+    ensures Spec.SplitIndex(old(I(node)), I(node), I(right), wit, pivot)
     ensures node.contents.nchildren == nleft
     ensures pivot == old(node.contents.pivots[nleft-1])
     modifies node
@@ -408,21 +415,21 @@ abstract module MutableBtree {
     SubReprsDisjoint(node, 0, nleft as int, nleft as int, node.contents.nchildren as int);
     right := SubIndex(node, nleft, node.contents.nchildren);
     pivot := node.contents.pivots[nleft-1];
-    assert BS.WF(I(node));
-    assert BS.AllKeys(I(node).children[0]) != {};
+    assert Spec.WF(I(node));
+    assert Spec.AllKeys(I(node).children[0]) != {};
     assert I(node).children[0] == I(node.contents.children[0]);
-    assert BS.AllKeys(I(node.contents.children[0])) != {};
-    wit :| wit in BS.AllKeys(I(node.contents.children[0]));
+    assert Spec.AllKeys(I(node.contents.children[0])) != {};
+    wit :| wit in Spec.AllKeys(I(node.contents.children[0]));
     IndexPrefix(node, nleft);
     ghost var inode := old(I(node));
     ghost var ileft := I(node);
     ghost var iright := I(right);
-    assert BS.AllKeysBelowBound(inode, 0);
-    BS.Keys.IsStrictlySortedImpliesLte(old(I(node)).pivots, 0, (nleft - 1) as int);
-    assert BS.Keys.lt(wit, inode.pivots[0]);
-    assert BS.Keys.lte(inode.pivots[0], pivot);
-    assert BS.Keys.lt(wit, pivot);
-    assert wit in BS.AllKeys(inode);
+    assert Spec.AllKeysBelowBound(inode, 0);
+    Spec.Keys.IsStrictlySortedImpliesLte(old(I(node)).pivots, 0, (nleft - 1) as int);
+    assert Spec.Keys.lt(wit, inode.pivots[0]);
+    assert Spec.Keys.lte(inode.pivots[0], pivot);
+    assert Spec.Keys.lt(wit, pivot);
+    assert wit in Spec.AllKeys(inode);
   }
   
   method SplitNode(node: Node) returns (right: Node, ghost wit: Key, pivot: Key)
@@ -437,14 +444,14 @@ abstract module MutableBtree {
     ensures node.repr !! right.repr
     ensures !Full(node)
     ensures !Full(right)
-    ensures BS.SplitNode(old(I(node)), I(node), I(right), wit, pivot)
-    ensures pivot in BS.AllKeys(old(I(node)))
+    ensures Spec.SplitNode(old(I(node)), I(node), I(right), wit, pivot)
+    ensures pivot in Spec.AllKeys(old(I(node)))
     modifies node
   {
     if node.contents.Leaf? {
       var boundary := node.contents.nkeys/2;
       pivot := node.contents.keys[boundary];
-      BS.Keys.IsStrictlySortedImpliesLt(node.contents.keys[..node.contents.nkeys], boundary as int - 1, boundary as int);
+      Spec.Keys.IsStrictlySortedImpliesLt(node.contents.keys[..node.contents.nkeys], boundary as int - 1, boundary as int);
       right, wit := SplitLeaf(node, node.contents.nkeys / 2, pivot);
     } else {
       var boundary := node.contents.nchildren/2;
@@ -626,10 +633,10 @@ abstract module MutableBtree {
     ensures node.contents.Index?
     ensures fresh(node.repr - old(node.repr))
     ensures node.height == old(node.height)
-    ensures BS.SplitChildOfIndex(old(I(node)), I(node), childidx as int, wit)
+    ensures Spec.SplitChildOfIndex(old(I(node)), I(node), childidx as int, wit)
     ensures !Full(node.contents.children[childidx])
     ensures !Full(node.contents.children[childidx+1])
-    ensures node.contents.pivots[childidx] in BS.AllKeys(old(I(node)).children[childidx])
+    ensures node.contents.pivots[childidx] in Spec.AllKeys(old(I(node)).children[childidx])
     modifies node, node.contents.pivots, node.contents.children, node.contents.children[childidx]
   {
     ChildrenAreDistinct(node);
@@ -677,13 +684,13 @@ abstract module MutableBtree {
     requires !Full(node)
     ensures WFShape(node)
     ensures node.repr == old(node.repr)
-    ensures I(node) == BS.InsertLeaf(old(I(node)), key, value)
-    ensures BS.WF(I(node))
-    ensures BS.Interpretation(I(node)) == BS.Interpretation(old(I(node)))[key := value]
-    ensures BS.AllKeys(I(node)) == BS.AllKeys(old(I(node))) + {key}
+    ensures I(node) == Spec.InsertLeaf(old(I(node)), key, value)
+    ensures Spec.WF(I(node))
+    ensures Spec.Interpretation(I(node)) == Spec.Interpretation(old(I(node)))[key := value]
+    ensures Spec.AllKeys(I(node)) == Spec.AllKeys(old(I(node))) + {key}
     modifies node, node.contents.keys, node.contents.values
   {
-    var posplus1: uint64 := BS.Keys.ArrayLargestLtePlus1(node.contents.keys, 0, node.contents.nkeys, key);
+    var posplus1: uint64 := Spec.Keys.ArrayLargestLtePlus1(node.contents.keys, 0, node.contents.nkeys, key);
     if 1 <= posplus1 && node.contents.keys[posplus1-1] == key {
       node.contents.values[posplus1-1] := value;
     } else {
@@ -691,7 +698,7 @@ abstract module MutableBtree {
       Arrays.Insert(node.contents.values, node.contents.nkeys, value, posplus1);
       node.contents := node.contents.(nkeys := node.contents.nkeys + 1);
     }
-    BS.InsertLeafIsCorrect(old(I(node)), key, value);
+    Spec.InsertLeafIsCorrect(old(I(node)), key, value);
   }
 
   twostate lemma InsertIndexChildNotFullPreservesWFShape(node: Node, childidx: int)
@@ -770,14 +777,14 @@ abstract module MutableBtree {
   method InsertIndexChildNotFull(node: Node, childidx: uint64, key: Key, value: Value)
     requires WF(node)
     requires node.contents.Index?
-    requires childidx as int == BS.Keys.LargestLte(node.contents.pivots[..node.contents.nchildren-1], key) + 1
+    requires childidx as int == Spec.Keys.LargestLte(node.contents.pivots[..node.contents.nchildren-1], key) + 1
     requires !Full(node.contents.children[childidx])
     ensures WFShape(node)
     ensures fresh(node.repr - old(node.repr))
     ensures node.height == old(node.height)
-    ensures BS.WF(I(node))
-    ensures BS.Interpretation(I(node)) == BS.Interpretation(old(I(node)))[key := value]
-    ensures BS.AllKeys(I(node)) <= BS.AllKeys(old(I(node))) + {key}
+    ensures Spec.WF(I(node))
+    ensures Spec.Interpretation(I(node)) == Spec.Interpretation(old(I(node)))[key := value]
+    ensures Spec.AllKeys(I(node)) <= Spec.AllKeys(old(I(node))) + {key}
     modifies node, node.contents.children[childidx], node.contents.children[childidx].repr
     decreases node.height, 0
   {
@@ -802,7 +809,7 @@ abstract module MutableBtree {
       assert old(DisjointSubtrees(node.contents, childidx as int, i as int));
     }
 
-    BS.RecursiveInsertIsCorrect(oldinode, key, value, childidx as int, inode, inode.children[childidx]);
+    Spec.RecursiveInsertIsCorrect(oldinode, key, value, childidx as int, inode, inode.children[childidx]);
   }
 
   method InsertIndexSelectAndPrepareChild(node: Node, key: Key) returns (childidx: uint64)
@@ -812,33 +819,33 @@ abstract module MutableBtree {
     ensures WFShape(node)
     ensures fresh(node.repr - old(node.repr))
     ensures node.height == old(node.height)
-    ensures BS.WF(I(node))
+    ensures Spec.WF(I(node))
     ensures node.contents.Index?
-    ensures childidx as int == BS.Keys.LargestLte(node.contents.pivots[..node.contents.nchildren-1], key) + 1
+    ensures childidx as int == Spec.Keys.LargestLte(node.contents.pivots[..node.contents.nchildren-1], key) + 1
     ensures !Full(node.contents.children[childidx])
-    ensures BS.Interpretation(I(node)) == BS.Interpretation(old(I(node)))
-    ensures BS.AllKeys(I(node)) == BS.AllKeys(old(I(node)))
+    ensures Spec.Interpretation(I(node)) == Spec.Interpretation(old(I(node)))
+    ensures Spec.AllKeys(I(node)) == Spec.AllKeys(old(I(node)))
     modifies node, node.repr
   {
-    childidx := BS.Keys.ArrayLargestLtePlus1(node.contents.pivots, 0, node.contents.nchildren-1, key);
+    childidx := Spec.Keys.ArrayLargestLtePlus1(node.contents.pivots, 0, node.contents.nchildren-1, key);
     if Full(node.contents.children[childidx]) {
       ghost var oldpivots := node.contents.pivots[..node.contents.nchildren-1];
       var wit := SplitChildOfIndex(node, childidx);
       ghost var newpivots := node.contents.pivots[..node.contents.nchildren-1];
-      BS.SplitChildOfIndexPreservesWF(old(I(node)), I(node), childidx as int, wit);
-      BS.SplitChildOfIndexPreservesInterpretation(old(I(node)), I(node), childidx as int, wit);
-      BS.SplitChildOfIndexPreservesAllKeys(old(I(node)), I(node), childidx as int, wit);
+      Spec.SplitChildOfIndexPreservesWF(old(I(node)), I(node), childidx as int, wit);
+      Spec.SplitChildOfIndexPreservesInterpretation(old(I(node)), I(node), childidx as int, wit);
+      Spec.SplitChildOfIndexPreservesAllKeys(old(I(node)), I(node), childidx as int, wit);
 
-      var t: int32 := BS.Keys.cmp(node.contents.pivots[childidx], key);
+      var t: int32 := Spec.Keys.cmp(node.contents.pivots[childidx], key);
       if  t <= 0 {
         childidx := childidx + 1;
         forall i | childidx as int - 1 < i < |newpivots|
-          ensures BS.Keys.lt(key, newpivots[i])
+          ensures Spec.Keys.lt(key, newpivots[i])
         {
           assert newpivots[i] == oldpivots[i-1];
         }
       }
-      BS.Keys.LargestLteIsUnique(node.contents.pivots[..node.contents.nchildren-1], key, childidx as int - 1);
+      Spec.Keys.LargestLteIsUnique(node.contents.pivots[..node.contents.nchildren-1], key, childidx as int - 1);
     }
   }
   
@@ -849,9 +856,9 @@ abstract module MutableBtree {
     ensures WFShape(node)
     ensures fresh(node.repr - old(node.repr))
     ensures node.height == old(node.height)
-    ensures BS.WF(I(node))
-    ensures BS.Interpretation(I(node)) == BS.Interpretation(old(I(node)))[key := value]
-    ensures BS.AllKeys(I(node)) <= BS.AllKeys(old(I(node))) + {key}
+    ensures Spec.WF(I(node))
+    ensures Spec.Interpretation(I(node)) == Spec.Interpretation(old(I(node)))[key := value]
+    ensures Spec.AllKeys(I(node)) <= Spec.AllKeys(old(I(node))) + {key}
     modifies node, node.repr
     decreases node.height, 1
   {
@@ -865,9 +872,9 @@ abstract module MutableBtree {
     ensures WFShape(node)
     ensures fresh(node.repr - old(node.repr))
     ensures node.height == old(node.height)
-    ensures BS.WF(I(node))
-    ensures BS.Interpretation(I(node)) == BS.Interpretation(old(I(node)))[key := value]
-    ensures BS.AllKeys(I(node)) <= BS.AllKeys(old(I(node))) + {key}
+    ensures Spec.WF(I(node))
+    ensures Spec.Interpretation(I(node)) == Spec.Interpretation(old(I(node)))[key := value]
+    ensures Spec.AllKeys(I(node)) <= Spec.AllKeys(old(I(node))) + {key}
     modifies node, node.repr
     decreases node.height, 2
   {
@@ -884,7 +891,7 @@ abstract module MutableBtree {
     ensures WFShape(newroot)
     ensures fresh(newroot.repr - root.repr)
     ensures newroot.height == root.height + 1
-    ensures I(newroot) == BS.Grow(I(root))
+    ensures I(newroot) == Spec.Grow(I(root))
     ensures !Full(newroot)
   {
     newroot := new Node;
@@ -902,13 +909,13 @@ abstract module MutableBtree {
   lemma FullImpliesAllKeysNonEmpty(node: Node)
     requires WF(node)
     requires Full(node)
-    ensures BS.AllKeys(I(node)) != {}
+    ensures Spec.AllKeys(I(node)) != {}
   {
     var inode := I(node);
     if inode.Leaf? {
-      assert inode.keys[0] in BS.AllKeys(inode);
+      assert inode.keys[0] in Spec.AllKeys(inode);
     } else {
-      assert inode.pivots[0] in BS.AllKeys(inode);
+      assert inode.pivots[0] in Spec.AllKeys(inode);
     }
   }
   
@@ -916,24 +923,24 @@ abstract module MutableBtree {
     requires WF(root)
     ensures WF(newroot)
     ensures fresh(newroot.repr - old(root.repr))
-    ensures BS.Interpretation(I(newroot)) == BS.Interpretation(old(I(root)))[key := value]
-    modifies root, root.repr
+    ensures Interpretation(newroot) == old(Interpretation(root))[key := value]
+    modifies root.repr
   {
     if Full(root) {
       FullImpliesAllKeysNonEmpty(root);
-      BS.GrowPreservesWF(I(root));
+      Spec.GrowPreservesWF(I(root));
       newroot := Grow(root);
     } else {
       newroot := root;
     }
-    assert BS.Interpretation(I(newroot)) == BS.Interpretation(old(I(root)));
+    assert Spec.Interpretation(I(newroot)) == Spec.Interpretation(old(I(root)));
     InsertNode(newroot, key, value);
   }
 
   method EmptyTree() returns (root: Node)
     ensures WF(root)
     ensures fresh(root.repr)
-    ensures BS.Interpretation(I(root)) == map[]
+    ensures Interpretation(root) == map[]
   {
     var rootkeys := newArrayFill(MaxKeysPerLeaf(), DefaultKey());
     var rootvalues := newArrayFill(MaxKeysPerLeaf(), DefaultValue());
@@ -952,7 +959,7 @@ module TestBtreeSpec refines BtreeSpec {
 }
 
 module TestMutableBtree refines MutableBtree {
-  import BS = TestBtreeSpec
+  import Spec = TestBtreeSpec
     
   function method MaxKeysPerLeaf() : uint64 { 64 }
   function method MaxChildren() : uint64 { 64 }
@@ -963,7 +970,7 @@ module TestMutableBtree refines MutableBtree {
 
 module MainModule {
   import opened NativeTypes
-  import TestMutableBtree
+  import TMB = TestMutableBtree`API
   
   method Main()
   {
@@ -973,16 +980,14 @@ module MainModule {
     var p: uint64 := 3_000_017;
     // var n: uint64 := 100_000_000;
     // var p: uint64 := 1_073_741_827;
-    var t := TestMutableBtree.EmptyTree();
+    var t := TMB.EmptyTree();
     var i: uint64 := 0;
     while i < n
       invariant 0 <= i <= n
-      invariant TestMutableBtree.WFShape(t)
-      invariant TestMutableBtree.BS.WF(TestMutableBtree.I(t))
-      invariant fresh(t)
+      invariant TMB.WF(t)
       invariant fresh(t.repr)
     {
-      t := TestMutableBtree.Insert(t, ((i * p) % n), i);
+      t := TMB.Insert(t, ((i * p) % n), i);
       i := i + 1;
     }
 
